spec+proofs: consolidate maxIRQ definition in Platform.thy
On Arm architectures, maxIRQ defaulted to Kernel_Config.maxIRQ, while on
other architectures, it defaulted to Platform.L4VARCH.maxIRQ. This
caused divergence when attempting to make interfaces that work on all
architectures when arch-splitting Interrupt_R.

By forcing a Platform.L4VARCH.maxIRQ definition to exist on all
platforms as an numeral, and pointing it to Kernel_Config.maxIRQ on
architectures that have it, we can now point to the same constant on all
architectures in interfaces.

For the design spec, we keep the abbreviation confining maxIRQ to type
irq.

For CRefine, add maxIRQ_def to [simp] in ArchMove_R for Kernel_Config
architectures, in order to keep the proof as close to what it used to
be, which expected to only see Kernel_Config.maxIRQ.

Refine update is the minimal necessary to proceed to Interrupt_R
arch-split, where we can have a go at proper interfacing.

Signed-off-by: Rafal Kolanski <rafal.kolanski@proofcraft.systems>

spec/machine/ARM_HYP/Platform.thy
@@ -36,6 +36,10 @@ context Arch begin global_naming ARM_HYP
 value_type irq_len = Kernel_Config.irqBits (* IRQ_CNODE_SLOT_BITS *)
 type_synonym irq = "irq_len word"
 
+(* maxIRQ is defined via Kernel_Config on this architecture *)
+definition maxIRQ :: "'a::numeral" where
+  "maxIRQ \<equiv> Kernel_Config.maxIRQ"
+
 (* List of supported Arm platforms that support GICv3 or GICv2 *)
 definition isGICPlatform :: bool where
   "isGICPlatform \<equiv> \<not>(config_PLAT_OMAP3 \<or> config_PLAT_AM335X \<or> config_PLAT_BCM2837)"
@@ -139,5 +143,9 @@ definition irqVTimerEvent :: "irq" where
   "irqVTimerEvent  \<equiv> 27"
 
 end
+
+(* we want to use the Platform constant in the global context instead of the arch-specific one from
+   Kernel_Config *)
+arch_requalify_consts (aliasing) maxIRQ
 
 end
