proof/crefine/RISCV64/Delete_C.thy
@@ -897,7 +897,7 @@ lemma finaliseSlot_ccorres:
                                 arch_cap_has_cleanup'_def
                          split: option.split capability.splits)
           apply (auto dest!: ctes_of_valid'
-                       simp: valid_cap'_def Kernel_C.maxIRQ_def RISCV64.maxIRQ_def
+                       simp: valid_cap'_def Kernel_C.maxIRQ_def maxIRQ_def
                              unat_ucast word_le_nat_alt cleanup_info_wf'_def arch_cleanup_info_wf'_def)[1]
          subgoal by (auto dest!: valid_capAligned ctes_of_valid'
                           simp: isCap_simps final_matters'_def o_def)
