proof/crefine/RISCV64/Finalise_C.thy
@@ -2187,7 +2187,7 @@ lemma finaliseCap_ccorres:
    apply (rule ccorres_if_lhs)
     apply (simp add: Collect_False Collect_True Let_def
                 del: Collect_const)
-    apply (rule_tac P="(capIRQ cap) \<le>  RISCV64.maxIRQ" in ccorres_gen_asm)
+    apply (rule_tac P="(capIRQ cap) \<le> maxIRQ" in ccorres_gen_asm)
     apply (rule ccorres_rhs_assoc)+
     apply csymbr
     apply csymbr
